refactoring

Network_Security_Policy_Verification/Examples/Impl_List_Playground_ChairNetwork.thy
@@ -21,7 +21,7 @@ text{*Our access control view on the network*}
 section{*Our security requirements*}
   subsection{*We have a server with confidential data*}
     definition ConfidentialChairData::"(vString NetworkSecurityModel)" where
-      "ConfidentialChairData \<equiv> new_configured_list_NetworkSecurityModel NM_BLPtrusted_impl.NM_LIB_BLPtrusted \<lparr> 
+      "ConfidentialChairData \<equiv> new_configured_list_NetworkSecurityModel SINVAR_BLPtrusted_impl.SINVAR_LIB_BLPtrusted \<lparr> 
           node_properties = [V ''FilesSrv'' \<mapsto> \<lparr> privacy_level = 1, trusted = False \<rparr>,
                              V ''Employees'' \<mapsto> \<lparr> privacy_level = 0, trusted = True \<rparr>,
                              V ''EReachable'' \<mapsto> \<lparr> privacy_level = 0, trusted = True \<rparr>], 
@@ -40,17 +40,17 @@ section{*Our security requirements*}
               Department ''BwPrinting'' [
                   Department ''Printer'' []]]"
     definition PrintingHierarchy::"vString NetworkSecurityModel" where
-      "PrintingHierarchy \<equiv> new_configured_list_NetworkSecurityModel NM_DomainHierarchyNG_impl.NM_LIB_DomainHierarchyNG \<lparr> 
+      "PrintingHierarchy \<equiv> new_configured_list_NetworkSecurityModel SINVAR_DomainHierarchyNG_impl.SINVAR_LIB_DomainHierarchyNG \<lparr> 
         node_properties = PrintingHierarchy_nodes,
         model_global_properties = PrintingHierarchy_tree
         \<rparr>"
   
     --"verify globals, I admit, not very elegant"
-    lemma "nm_verify_globals NM_DomainHierarchyNG_impl.NM_LIB_DomainHierarchyNG ChairNetwork_empty 
-          (nm_node_props NM_DomainHierarchyNG_impl.NM_LIB_DomainHierarchyNG \<lparr> node_properties = PrintingHierarchy_nodes, model_global_properties = PrintingHierarchy_tree \<rparr>) PrintingHierarchy_tree" by eval
+    lemma "nm_verify_globals SINVAR_DomainHierarchyNG_impl.SINVAR_LIB_DomainHierarchyNG ChairNetwork_empty 
+          (nm_node_props SINVAR_DomainHierarchyNG_impl.SINVAR_LIB_DomainHierarchyNG \<lparr> node_properties = PrintingHierarchy_nodes, model_global_properties = PrintingHierarchy_tree \<rparr>) PrintingHierarchy_tree" by eval
   *)
   subsection{* The color printer is only accessibly by employees, The black.white printer by employees and students*}
-    definition "PrintingACL \<equiv> new_configured_list_NetworkSecurityModel NM_LIB_CommunicationPartners \<lparr> 
+    definition "PrintingACL \<equiv> new_configured_list_NetworkSecurityModel SINVAR_LIB_CommunicationPartners \<lparr> 
           node_properties = [V ''PrinterColor'' \<mapsto> Master [V ''Employees'', V ''EReachable''],
                              V ''PrinterBW'' \<mapsto> Master [V ''Employees'', V ''EReachable'', V ''Students''],
                              V ''Employees'' \<mapsto> Care,
@@ -60,7 +60,7 @@ section{*Our security requirements*}
           \<rparr>"
 
   subsection{* Printers are information sinks *}
-    definition "PrintingSink \<equiv> new_configured_list_NetworkSecurityModel NM_LIB_Sink \<lparr> 
+    definition "PrintingSink \<equiv> new_configured_list_NetworkSecurityModel SINVAR_LIB_Sink \<lparr> 
           node_properties = [V ''PrinterColor'' \<mapsto> Sink,
                              V ''PrinterBW'' \<mapsto> Sink], 
           model_global_properties = () 
@@ -69,14 +69,14 @@ section{*Our security requirements*}
 
 
   subsection{*Students may access each other but are not accessible from the outside*}
-    definition "StudentSubnet \<equiv> new_configured_list_NetworkSecurityModel NM_LIB_SubnetsInGW \<lparr> 
+    definition "StudentSubnet \<equiv> new_configured_list_NetworkSecurityModel SINVAR_LIB_SubnetsInGW \<lparr> 
           node_properties = [V ''Students'' \<mapsto> Member, V ''Employees'' \<mapsto> Member, V ''EReachable'' \<mapsto> InboundGateway], 
           model_global_properties = () 
           \<rparr>"
 
 
   subsection{* The files server is only accessibly by employees*}
-    definition "FilesSrcACL \<equiv> new_configured_list_NetworkSecurityModel NM_LIB_CommunicationPartners \<lparr> 
+    definition "FilesSrcACL \<equiv> new_configured_list_NetworkSecurityModel SINVAR_LIB_CommunicationPartners \<lparr> 
           node_properties = [V ''FilesSrv'' \<mapsto> Master [V ''Employees'', V ''EReachable''],
                              V ''Employees'' \<mapsto> Care,
                              V ''EReachable'' \<mapsto> Care], 
