Network_Security_Policy_Verification/Network_Security_Policy_Verification.thy
@@ -1,5 +1,6 @@
 theory Network_Security_Policy_Verification
 imports
+  TopoS_Interface
   TopoS_Library
   TopoS_Composition_Theory
   TopoS_Stateful_Policy
