Network_Security_Policy_Verification/TopoS_Library.thy
@@ -1,22 +1,22 @@
 theory TopoS_Library
 imports String 
   "Lib/FiniteListGraph_Impl"
-  "Security_Invariants/NM_BLPbasic_impl"
-  "Security_Invariants/NM_Subnets_impl"
-  "Security_Invariants/NM_DomainHierarchyNG_impl"
-  "Security_Invariants/NM_BLPtrusted_impl"
-  (*"Security_Invariants/NM_SecurityGateway_impl"*) (*deprecated, will be removed*)
-  "Security_Invariants/NM_SecGwExt_impl"
-  "Security_Invariants/NM_Sink_impl"
-  "Security_Invariants/NM_SubnetsInGW_impl"
-  "Security_Invariants/NM_CommunicationPartners_impl"
-  "Security_Invariants/NM_NoRefl_impl"
+  "Security_Invariants/SINVAR_BLPbasic_impl"
+  "Security_Invariants/SINVAR_Subnets_impl"
+  "Security_Invariants/SINVAR_DomainHierarchyNG_impl"
+  "Security_Invariants/SINVAR_BLPtrusted_impl"
+  (*"Security_Invariants/SINVAR_SecurityGateway_impl"*) (*deprecated, will be removed*)
+  "Security_Invariants/SINVAR_SecGwExt_impl"
+  "Security_Invariants/SINVAR_Sink_impl"
+  "Security_Invariants/SINVAR_SubnetsInGW_impl"
+  "Security_Invariants/SINVAR_CommunicationPartners_impl"
+  "Security_Invariants/SINVAR_NoRefl_impl"
   (*invariants you probably don't wat to use because of exponential runtime*)
-  "Security_Invariants/NM_Dependability_impl"
-  "Security_Invariants/NM_NonInterference_impl"
-  "Security_Invariants/NM_ACLnotCommunicateWith_impl"
-  "Security_Invariants/NM_ACLcommunicateWith_impl"
-  "Security_Invariants/NM_Dependability_norefl_impl"
+  "Security_Invariants/SINVAR_Dependability_impl"
+  "Security_Invariants/SINVAR_NonInterference_impl"
+  "Security_Invariants/SINVAR_ACLnotCommunicateWith_impl"
+  "Security_Invariants/SINVAR_ACLcommunicateWith_impl"
+  "Security_Invariants/SINVAR_Dependability_norefl_impl"
   "Lib/Efficient_Distinct"
   "~~/src/HOL/Library/Code_Target_Nat"
 begin
@@ -24,7 +24,7 @@ begin
 (* possibly include: "~~/src/HOL/Library/Code_Char_chr" "~~/src/HOL/Library/Efficient_Nat" *)
   
   
-(*none of those should be defined or a hide_const is missing at the end of a NM_*.thy file*)
+(*none of those should be defined or a hide_const is missing at the end of a SINVAR_*.thy file*)
 term sinvar
 term receiver_violation
 term verify_globals
@@ -36,19 +36,19 @@ term eval
 print_interps TopoS_modelLibrary
 
 (*some check: *)
-  thm NM_LIB_BLPbasic_interpretation.impl_spec
-  thm NM_LIB_Dependability_interpretation.impl_spec
-  thm NM_LIB_DomainHierarchyNG_interpretation.impl_spec
-  thm NM_LIB_Subnets_interpretation.impl_spec
-  thm NM_LIB_BLPtrusted_interpretation.impl_spec
-  (*thm NM_LIB_SecurityGateway_interpretation.impl_spec*)
-  thm NM_LIB_SecurityGatewayExtended_interpretation.impl_spec
-  thm NM_LIB_Sink_interpretation.impl_spec
-  thm NM_LIB_NonInterference_interpretation.impl_spec
-  thm NM_LIB_SubnetsInGW_interpretation.impl_spec
-  thm NM_LIB_CommunicationPartners_interpretation.impl_spec
-  thm NM_LIB_Dependability_interpretation.impl_spec
-  thm NM_LIB_ACLcommunicateWith_interpretation.impl_spec
+  thm SINVAR_LIB_BLPbasic_interpretation.impl_spec
+  thm SINVAR_LIB_Dependability_interpretation.impl_spec
+  thm SINVAR_LIB_DomainHierarchyNG_interpretation.impl_spec
+  thm SINVAR_LIB_Subnets_interpretation.impl_spec
+  thm SINVAR_LIB_BLPtrusted_interpretation.impl_spec
+  (*thm SINVAR_LIB_SecurityGateway_interpretation.impl_spec*)
+  thm SINVAR_LIB_SecurityGatewayExtended_interpretation.impl_spec
+  thm SINVAR_LIB_Sink_interpretation.impl_spec
+  thm SINVAR_LIB_NonInterference_interpretation.impl_spec
+  thm SINVAR_LIB_SubnetsInGW_interpretation.impl_spec
+  thm SINVAR_LIB_CommunicationPartners_interpretation.impl_spec
+  thm SINVAR_LIB_Dependability_interpretation.impl_spec
+  thm SINVAR_LIB_ACLcommunicateWith_interpretation.impl_spec
 
 
 (*nothing to see here, just loads all the models, ...*)
@@ -58,12 +58,12 @@ print_interps TopoS_modelLibrary
 
 section{*Example*}
   definition BLPexample1::"bool" where
-    "BLPexample1 \<equiv> (nm_eval NM_LIB_BLPbasic) fabNet \<lparr> node_properties = [TopoS_Vertices.V ''PresenceSensor'' \<mapsto> 2, 
+    "BLPexample1 \<equiv> (nm_eval SINVAR_LIB_BLPbasic) fabNet \<lparr> node_properties = [TopoS_Vertices.V ''PresenceSensor'' \<mapsto> 2, 
                                                     TopoS_Vertices.V ''Webcam'' \<mapsto> 3, 
                                                     TopoS_Vertices.V ''SensorSink'' \<mapsto> 3,
                                                     TopoS_Vertices.V ''Statistics'' \<mapsto> 3], model_global_properties = () \<rparr>"
   definition BLPexample3::"(vString \<times> vString) list list" where
-    "BLPexample3 \<equiv> (nm_offending_flows NM_LIB_BLPbasic) fabNet ((nm_node_props NM_LIB_BLPbasic) sensorProps_NMParams_try3)"
+    "BLPexample3 \<equiv> (nm_offending_flows SINVAR_LIB_BLPbasic) fabNet ((nm_node_props SINVAR_LIB_BLPbasic) sensorProps_NMParams_try3)"
 
   value[code] "BLPexample1"
   value[code] "BLPexample3"
